Update Spec.
1. Change Ballot type from Int to Nat. Int is simply wrong since it's
   not bounded below. It was used to accommodate the -1 (empty ballot)
used in the TLA proof.
2. Use `none` (Option Ballot) to represent the empty ballot, also the
   empty value. As a consequence, need to change twob to use Option
Ballot and Option Value to make it compatible in the defintion of
max_prop.
3. Change the variable name in Phase2a (maxV -> maxVBal). maxV is just
   unclear.

Paxos/Spec.lean
@@ -6,18 +6,70 @@ open Classical
 
 -- Types Definition --
 abbrev Acceptor := String   -- Acceptor
-abbrev Value := Nat         -- Value
-abbrev Ballot := Int        -- Ballot is defined to be Int to include -1 as empty ballot
+abbrev Value := String      -- Value
+abbrev Ballot := Nat        -- Ballot is defined to be Nat. We model the empty ballot (defined as -1 in the TLA proof) as none (Option Ballot).
 
--- Special Ballot (empty) --
-abbrev ballot_neg_one := -1
+-- Define +, < between Ballot and Option Ballot --
+instance : HAdd (Option Ballot) Ballot (Option Ballot) where
+  hAdd
+    | none,    0      => none         -- -1 + 0     = -1
+    | none,    Nat.succ k => k        -- 0  + (k+1) = k
+    | some a,  b      => a + b        -- a  +  b    = a + b
+
+instance : HAdd (Option Ballot) Nat (Option Ballot) where       -- TODO: can this be removed?
+  hAdd
+    | none,    0      => none         -- -1 + 0     = -1
+    | none,    Nat.succ k => k        -- 0  + (k+1) = k
+    | some a,  b      => a + b        -- a  +  b    = a + b
+
+instance : LE (Option Ballot) where
+  le
+    | none,    _        => True
+    | some _,  none     => False
+    | some a,  some b   => a ≤ b
+
+@[instance]
+instance : LT (Option Ballot) where
+  lt
+    | none,    _        => True
+    | some _,  none     => False
+    | some a,  some b   => a < b
+
+instance decidableLeOption {x y : Option Ballot} : Decidable (x ≤ y) :=
+  match x, y with
+  | none,    _        => isTrue (by trivial)
+  | some _,  none     => isFalse (by exact fun a ↦ a)
+  | some a,  some b   => inferInstance
+
+instance decidableLtOption {x y : Option Ballot} : Decidable (x < y) :=
+  match x, y with
+  | none,    _        => isTrue (by trivial)
+  | some _,  none     => isFalse (by exact fun a ↦ a)
+  | some a,  some b   => inferInstance
+
+-- Examples of using the defined operations on Ballot and Option Ballot
+-- #eval (none: Option Ballot) + (1: Ballot)
+-- #eval (0: Ballot) ≤ (1: Ballot)
+-- #eval (some 0: Option Ballot) ≤ (some 1: Option Ballot)
+-- #eval (none: Option Ballot) + 1 ≤ (none: Option Ballot)
+
+-- Minimal example, I was trying to prove this using linarith but it didn't work. This is used to prove the inductiveness of Phase 2a.
+example {b b1: Ballot} (h1: b1 ≤ b) (h2: b ≤ b1 - 1) (h3: b1 > 0) : False := by
+  have h2' : b < b1 := by exact (Nat.lt_iff_le_pred h3).mpr h2
+  have hf : b1 < b1 := by exact Nat.lt_of_le_of_lt h1 h2'
+  simp at hf
+
+@[simp]
+theorem ballot_none_plus_one_leq_ballot {b : Ballot} : (none : Option Ballot) + (1 : Ballot) ≤ some b := by
+  dsimp [HAdd.hAdd]
+  exact Nat.zero_le b
 
 -- We define Message as an inductive type --
 inductive Message where
 | onea  (bal : Ballot) : Message
-| oneb  (bal : Ballot) (maxVBal : Ballot) (maxVal : Option Value) (acc : Acceptor) : Message -- maxVBal could be 0, and maxVal could be none
+| oneb  (bal : Ballot) (maxVBal : Option Ballot) (maxVal : Option Value) (acc : Acceptor) : Message --  Define both Ballot and Value to be Option type, corresponds to not voted.
 | twoa  (bal : Ballot) (val : Value) : Message
-| twob  (bal : Ballot) (val : Option Value) (acc : Acceptor) : Message                       -- val is of Option becuase last_voted defintion
+| twob  (bal : Option Ballot) (val : Option Value) (acc : Acceptor) : Message                       -- val is of Option becuase last_voted defintion
 
 /-  Line 16 - 18
 ASSUME QuorumAssumption ==
@@ -38,7 +90,7 @@ variable (sent sent': Set Message) -- sent' is added here to model the next stat
 Send(m) == sent' = sent \cup {m}
 -/
 @[simp]
-def Send (m : Message) (sent₁ : Set Message) := sent₁ ∪ {m}
+def Send (m : Message) (sent : Set Message) := sent ∪ {m}
 
 /- Line 30
 Init == sent = {} -/
@@ -57,11 +109,31 @@ However, instead of returning a tuple for the ballot and value, we return a set 
 Note: last_voted(a) is used in the [github repo](https://github.com/DistAlgo/proofs/blob/master/basic-paxos/PaxosHistVarNFM18.tla#L47). However, in the paper (https://arxiv.org/pdf/1802.09687), the name is max_prop. Here we use max_prop because it is more informative.
 -/
 def max_prop (a : Acceptor): Set Message :=
-  let twobs := {m ∈ sent | ∃ b v, m = Message.twob b v a}
+  let twobs := {m ∈ sent | ∃ (b: Ballot) (v: Value), m = Message.twob b v a}          -- The twob messages should have concrete ballot and value, not Option type. We explicitly write out the types.
   if twobs ≠ ∅ then
-    { m₁ ∈ twobs | ∀m₂ ∈ twobs, ∃ b₁ b₂ v₁ v₂,
+    { m₁ ∈ twobs | ∀m₂ ∈ twobs, ∃ (b₁ b₂: Ballot) (v₁ v₂: Value),                     -- Same as above
       m₁ = Message.twob b₁ v₁ a ∧ m₂ = Message.twob b₂ v₂ a ∧ b₁ ≥ b₂}
-  else {Message.twob (-1) none a}
+  else {Message.twob none none a}                                                     -- For -1 ballot, we use `none`. At the same time, returning `none` as the value.
+
+-- Effort: 20 min
+/-- This lemma states that either one of ballot or value is empty, then the other one must also be empty
+
+This is used in later proof when we need to do
+
+`match rbal, rval with
+| some rbal, none | none, some rval => `
+
+and derives a contradiction because it can't be the case.
+-/
+@[simp]
+lemma max_prop_empty_ballot_iff_empty_value {a : Acceptor} {m : Message}
+  (hm : m ∈ max_prop sent a) :
+  (∃ b, m = Message.twob (some b) none a) ↔ ∃ v, m = Message.twob none (some v) a := by
+  dsimp [max_prop] at hm
+  let twobs := { m | m ∈ sent ∧ ∃ b v, m = Message.twob (some b) (some v) a }
+  split_ifs at hm with h_nonempty
+  · simp at hm; simp [hm];
+  · simp [*] at hm; have h_m_twob := hm.left.right; rcases h_m_twob with ⟨b, v, rfl⟩; simp;
 
 /-- Phase 1b: For an acceptor a, if there is a 1a message m with ballot m.bal that is higher than the highest it
 has seen, a sends a 1b message with m.bal alongwith the highest-numbered pair it has voted for.
@@ -73,12 +145,12 @@ In first order logic we would write this as: `(A → B) ∧ (¬A → C)`, where 
 def Phase1b (a : Acceptor) : Prop :=
   ∃ m ∈ sent, ∃r ∈ max_prop sent a,
     match m, r with
-    | Message.onea b, Message.twob rbal rval _a => -- max_prop_bal might be -1 and max_prop_val could be none
+    | Message.onea b, Message.twob rbal rval _a =>          -- rbal and rval are Option type, they could both be none.
        if (∀m2 ∈ sent, match m2 with
        | Message.oneb b2 _ _ a' => (a' = a) → (b > b2)
        | Message.twob b2 _ a' => (a' = a) → (b > b2)
        | _ => True)
-       then sent' = Send (Message.oneb b rbal rval a) sent
+       then sent' = Send (Message.oneb b rbal rval a) sent  -- rbal and rval are Option type, they could both be none.
        else sent' = sent
     | _, _ => False
 
@@ -94,12 +166,12 @@ def Phase2a (b : Ballot) : Prop :=
                 | _                 => False)
   then
     if φ : ∃ (v : Value) (Q : Set Acceptor) (S : Set Message), Q ∈ Quorums ∧ S ⊆ { m ∈ sent | match m with | Message.oneb b' _ _ _ => b' = b | _ => False}  -- S is the set of 1b messages with ballot b
-      ∧ (∀ a ∈ Q, ∃ m ∈ S, match m with | Message.oneb _ _ _ a' => a' = a | _ => False)     -- for all acceptors in Q, there is a corresponding 1b message in S.
-      ∧ ((∀ m ∈ S, match m with | Message.oneb _ maxV _ _ => maxV = -1 | _ => True)         -- for all 1b messages, either that maxVal is -1 (no acceptor has voted for anything)
-          ∨ ∃ (c : Ballot), 0 ≤ c ∧ c ≤ b - 1                                               -- or there is a 1b message with ballot c (the 'highest ballot') that is less than b
-              ∧ (∀ m ∈ S, match m with | Message.oneb _ maxV _ _ => maxV ≤ c | _ => True)   -- and for all 1b messages, the maxV is less than or equal to c
-              ∧ (∃ m ∈ S, match m with | Message.oneb _ maxV maxVal _ => maxV = c ∧ maxVal = v | _ => False)) -- and there is a 1b message with ballot c and value v
-    then let v := choose φ; sent' = Send (Message.twoa b v) sent
+      ∧ (∀ a ∈ Q, ∃ m ∈ S, match m with | Message.oneb _ _ _ a' => a' = a | _ => False)         -- for all acceptors in Q, there is a corresponding 1b message in S.
+      ∧ ((∀ m ∈ S, match m with | Message.oneb _ maxVBal _ _ => maxVBal = none | _ => True)     -- for all 1b messages, either that maxVal is -1 (no acceptor has voted for anything)
+          ∨ ∃ (c : Ballot), 0 ≤ c ∧ c ≤ b - (1 : Nat)                                             -- or there is a 1b message with ballot c (the 'highest ballot') that is less than b
+              ∧ (∀ m ∈ S, match m with | Message.oneb _ maxVBal _ _ => maxVBal ≤ c | _ => True)   -- and for all 1b messages, the maxV is less than or equal to c
+              ∧ (∃ m ∈ S, match m with | Message.oneb _ maxVBal maxVal _ => maxVBal = c ∧ maxVal = v | _ => False)) -- and there is a 1b message with ballot c and value v
+    then let v := choose φ; sent' = Send (Message.twoa b v) sent                                -- because `φ` is true, we can choose such value `v`.
     else
       sent' = sent
   else
